align $q$ to z-axis:
\begin{align}
q &= (q_0,0,0,q_z,\hat 0)\\
k_1 &= (\omega_1,0,\abs{\vec p_2}\sin\psi,\abs{\vec p_2}\cos\psi-q_z, \hat 0)\\
p_2 &= (E_2,0,\abs{\vec p_2}\sin\psi,\abs{\vec p_2}\cos\psi, \hat 0)
\end{align}

constraints, from energy conservation, masses ($k_2^2 = 0$ is already fixed) and external Mandelstam variables:
\begin{align}
q_0+\omega_1 & &&=E_1+E_2+\omega_2 \label{eq:PSConIIMomCon}\\
m^2 &= p_1^2 &&= E_1^2 - \omega_2^2 \label{eq:PSConIIp1}\\
m^2 &= p_2^2 &&= E_2^2 - \abs{\vec p_2}^2 \label{eq:PSConIIp2} \\
q^2 & &&= q_0^2 - q_z^2 \label{eq:PSConIIq}\\
0 & &&= \omega_1^2 - \abs{\vec p_2}^2 + 2\abs{\vec p_2}q_z\cos\psi-q_z^2 \label{eq:PSConIIk1}\\
s &= (q+k_1)^2 &&= (q_0+\omega_1)^2 - \abs{\vec p_2}^2 \label{eq:PSConIIs}\\
t &= (k_1-p_2)^2 &&= (\omega_1-E_2)^2-q_z^2 \label{eq:PSConIIt}\\
u &= (q-p_2)^2 &&= (q_0-E_2)^2 - \abs{\vec p_2}^2+2\abs{\vec p_2}q_z\cos\psi - q_z^2 \label{eq:PSConIIu}
\end{align}

solve:
\begin{align}
(\ref{eq:PSConIIu})-(\ref{eq:PSConIIk1}) &= u=(q_0-E_2)^2-\omega_1^2 \label{eq:PSConIIu2}\\
(\ref{eq:PSConIIs}) - (\ref{eq:PSConIIq}) + (\ref{eq:PSConIIt}) - (\ref{eq:PSConIIp2}) + (\ref{eq:PSConIIu2}) &= s-q^2+t-m^2+u\\
 &= s_4+m^2 = (\omega_1+q_0-E_2)^2 \label{eq:PSConIIs4}\\
(\ref{eq:PSConIIt}) + (\ref{eq:PSConIIu}) - (\ref{eq:PSConIIq}) &= t+u-q^2 = 2(E_2-\omega_1-q_0)E_2\\
\Rightarrow E_2 &= -\frac{t+u-q^2}{2\sqrt{s_4+m^2}} =\frac{s-s_4-2m^2}{2\sqrt{s_4+m^2}} = (\ref{eq:PSConIE2}) \label{eq:PSConIIE2}\\
(\ref{eq:PSConIIs}) - (\ref{eq:PSConIIq}) + (\ref{eq:PSConIIt}) - (\ref{eq:PSConIIp2}) &= s-q^2+t-m^2 = -2(E_2-\omega_1-q_0)\omega_1\\
\Rightarrow \omega_1 &= \frac{s'+t_1}{2\sqrt{s_4+m^2}} =\frac{s_4-u_1}{2\sqrt{s_4+m^2}} = (\ref{eq:PSConIom1}) \label{eq:PSConIIom1}\\
(\ref{eq:PSConIIs4}) \land (\ref{eq:PSConIIE2}) \land (\ref{eq:PSConIIom1}) \Rightarrow q_0 &= \frac{s+u_1}{2\sqrt{s_4+m^2}} = (\ref{eq:PSConIq0}) \label{eq:PSConIIq0}\\
(\ref{eq:PSConIIs}) \land (\ref{eq:PSConIIq0}) \land (\ref{eq:PSConIIom1}) \Rightarrow \abs{\vec p_2} &= \frac{\sqrt{(s-s_4)^2-4m^2 s}}{2\sqrt{s_4+m^2}} = (\ref{eq:PSConIabsp2}) \label{eq:PSConIIabsp2}\\
(\ref{eq:PSConIIq}) \land (\ref{eq:PSConIIq0}) \Rightarrow q_z &= \frac{\sqrt{(s'+u_1')^2-4q^2t}}{2\sqrt{s_4+m^2}} \label{eq:PSConIIqz}\\
(\ref{eq:PSConIIp1}) \Rightarrow \omega_2 &= \frac{s_4}{2\sqrt{s_4+m^2}} = (\ref{eq:PSConIom2}) \label{eq:PSConIIom2}\\
(\ref{eq:PSConIIMomCon}) \Rightarrow E_1 &= \frac{s_4+2m^2}{2\sqrt{s_4+m^2}} = (\ref{eq:PSConIE1}) \label{eq:PSConIIE1}\\
(\ref{eq:PSConIIq}) \Rightarrow \cos\psi &= \frac{s(q^2-t-m^2)- 2q^2(s_4+m^2)+s_4 u_1}{\sqrt{((s-s_4)^2-4m^2s)((s'+u_1')^2-4q^2 t)}} \neq (\ref{eq:PSConIcospsi}) \label{eq:PSConIIcospsi}
\end{align}

\begin{align}
&&u' &=(q-k_2)^2 = q^2-2qk_2 &&= q^2-2(q_0\omega_2 -q_z\omega_2\cos\theta_1\\
&&u_7 &= q^2-2qp_1 &&=q^2 - 2(q_0E_1 +q_z\omega_2\cos\theta_1)\\
(\ref{eq:MomCon3wq}): &&0 &=s'+u_1'+u_7+u'\quad\checkmark
\end{align}

\begin{align}
&&s_3 &= 2k_2p_2 = 2\omega_2(E_2-\abs{\vec p_2}(\cos\psi\cos\theta_1+\sin\psi\sin\theta_1\cos\theta_2)) = (\ref{eq:PSConIs3})\\
&&s_5 &= (p_1+p_2)^2 = 2m^2+2p_1p_2\\
&& &= 2(m^2+E_1E_2+\omega_2\abs{\vec p_2}(\cos\psi\cos\theta_1+\sin\psi\sin\theta_1\cos\theta_2)) = (\ref{eq:PSConIs5})\\
(\ref{eq:MomCon3wp2}): &&0 &= s_3+s_5+t_1+u_1'\quad\checkmark
\end{align}

\begin{align}
&&t' &= -2k_1k_2\\
 &&&= -2\omega_2(\omega_1 - (\abs{\vec p_2}\cos\psi-q_z)\cos\theta_1 - \abs{\vec p_2}\sin\psi\sin\theta_1\cos\theta_2)\\
&&u_6 &= - 2k_1p_1\\
 &&&= -2(\omega_1 E_1 + \omega_2(\abs{\vec p_2}\cos\psi-q_z)\cos\theta_1 + \omega_2\abs{\vec p_2}\sin\psi\sin\theta_1\cos\theta_2)\\
(\ref{eq:MomCon3wk1}): &&0 &= s'+t_1+t'+u_6\quad\checkmark
\end{align}

same as before: $t'$ is the only variable that can get collinear (for $-q^2 > 0$) - now collinear as [ABC] variable.
