at phase space integration there occur integrations over propagators\cite{Bojak:2000eu,PhysRevD.40.54,van_neerven_dimensional_1986}; the propagators can be decomposed in 2 types: [ab] and [ABC]; the needed integrals then reduce to the master formula:
\begin{align}
I_n^{(k,l)} &=\int\limits_0^\pi\!d\theta_1\,\sin^{n-3}(\theta_1)\int\limits_0^\pi\!d\theta_2\,\sin^{n-4}(\theta_2)(a+b\cos(\theta_1))^{-k}(A+B\cos(\theta_1)+C\sin(\theta_1)\cos(\theta_2))^{-l}\\
&=\int\!d\Omega_n\,(a+b\cos(\theta_1))^{-k}(A+B\cos(\theta_1)+C\sin(\theta_1)\cos(\theta_2))^{-l}
\end{align}

the integrals can be further destinguished by the range of $k,l$ and the type of collinearity (following the notation in \cite{Bojak:2000eu}):
\begin{itemize}
\item "non collinear": $a^2\neq b^2 \land A^2 \neq B^2 + C^2 \rightarrow I_{0,n}^{(k,l)}$
\item "single collinear a": $a=-b \land A^2 \neq B^2 + C^2 \rightarrow I_{a,n}^{(k,l)}$
\item "single collinear A": $a^2\neq b^2 \land A^2 = B^2 + C^2 \rightarrow I_{A,n}^{(k,l)}$
\item "double collinear": $a=-b \land A = -\sqrt{B^2 + C^2} \rightarrow I_{aA,n}^{(k,l)}$
\end{itemize}

Use $n=4+\epsilon$.

\subsubsection{integral helper}
define helper integral
\begin{equation}
\hat I^{(q)}(\nu) := \int\limits_0^\pi\!dt\,\sin^{\nu-3}(t)\cos^{q}(t)
\end{equation}

It is\cite[eq. 5.12.6]{NIST:DLMF}:
\begin{equation}
\int_{0}^{\pi}(\mathop{\sin\/}\nolimits t)^{\alpha-1}e^{i\beta t}dt=\frac{\pi}{2^{\alpha-1}} \frac{e^{i\pi \beta/2}}{\alpha\mathop{B}\left((\alpha+\beta+1)/2,(\alpha-\beta+1)/2\right)} \qquad\text{if}\,\Re(\alpha) > 0
\end{equation}
\begin{align}
\Rightarrow \hat I^{(0)}(n) &= \frac{\pi}{2^{n-3}(n-2)}\frac 1 {\mathop{B}((n-1)/2,(n-1)/2)}\\
\Rightarrow \hat I^{(0)}(n-1) &= \frac{\pi}{2^{n-4}(n-3)}\frac 1 {\mathop{B}((n-2)/2,(n-2)/2)}=\mathop{B}((n-3)/2,1/2)
\end{align}

If q is odd: $\hat I^{(q)}=0$, due to symetry of kernel; if q is even: $q=2p$ with $p\in\mathbbm N$:
\begin{align}
\hat I^{(2p)}(\nu) &= \frac 1 {2^{2p}}\sum\limits_{k=0}^{2p} \binom{2p}{k} \int\limits_0^\pi\sin^{\nu-3}(t)\exp(2i(k-p)t)\,dt\\
 &= \frac \pi{2^{2p+\nu-3} (\nu-2)}\sum\limits_{k=0}^{2p} \binom{2p}{k}\frac{\exp(i\pi(k-p))}{\mathop{B}((\nu-1)/2+(k-p),(\nu-1)/2-(k-p))}\\
 &= \frac \pi{2^{2p+\nu-3} (\nu-2)}\sum\limits_{l=-p}^{p} \binom{2p}{p+l}\frac{(-1)^l}{\mathop{B}((\nu-1)/2+l,(\nu-1)/2-l)}\\
 &= \frac {\pi\Gamma(\nu-1)(2p)!}{2^{2p+\nu-3} (\nu-2)\Gamma(\frac{n-1} 2+p)\Gamma(\frac{n-1} 2+p)}\left(\frac 1 {(p!)^2} \frac{\Gamma(\frac{\nu-1} 2+p)}{\Gamma(\frac{\nu-1} 2)}\frac{\Gamma(\frac{\nu-1} 2-p)}{\Gamma(\frac{\nu-1} 2)} \right. \nonumber\\
 &\hspace{40pt}\left. + 2\sum\limits_{l=1}^{p}\frac{(-1)^l}{(p+l)!(p-l)!}\frac{\Gamma(\frac{\nu-1} 2+p)}{\Gamma(\frac{\nu-1} 2+l)}\frac{\Gamma(\frac{\nu-1} 2-p)}{\Gamma(\frac{\nu-1} 2-l)}\right)\\
 &= \frac {2^{3-\nu}\pi\Gamma(\nu-1)}{(\nu-2)\Gamma(\frac{n-1} 2+p)\Gamma(\frac{n-1} 2+p)}\cdot \frac{\Gamma(\frac{\nu-1} 2-p)}{2^{p}\Gamma(\frac{\nu-1} 2)} \cdot \frac{(2p)!}{2^p p!} \cdot p! \left(\frac 1 {(p!)^2} \frac{\Gamma(\frac{\nu-1} 2+p)}{\Gamma(\frac{\nu-1} 2)} \right. \nonumber\\
 &\hspace{40pt}\left. + 2\sum\limits_{l=1}^{p}\frac{(-1)^l}{(p+l)!(p-l)!}\frac{\Gamma(\frac{\nu-1} 2+p)}{\Gamma(\frac{\nu-1} 2+l)}\frac{\Gamma(\frac{\nu-1} 2)}{\Gamma(\frac{\nu-1} 2-l)}\right)
\end{align}
TODO: prove \fxerror{prove}
\begin{align}
&p! \left(\frac 1 {(p!)^2} \frac{\Gamma(\frac{\nu-1} 2+p)}{\Gamma(\frac{\nu-1} 2)} + 2\sum\limits_{l=1}^{p}\frac{(-1)^l}{(p+l)!(p-l)!}\frac{\Gamma(\frac{\nu-1} 2+p)}{\Gamma(\frac{\nu-1} 2+l)}\frac{\Gamma(\frac{\nu-1} 2)}{\Gamma(\frac{\nu-1} 2-l)}\right)\\
&= \frac {1} {p!}\frac{\Gamma(-\frac{1}2+p)}{\Gamma(-\frac{1}2)} + 2\sum\limits_{l=1}^{p}\frac{(-1)^l p!}{(p+l)!(p-l)!}\frac{\Gamma(-\frac{1} 2+p)}{\Gamma(-\frac{1} 2+l)}\frac{\Gamma(-\frac{1} 2)}{\Gamma(-\frac{1} 2-l)}\\
&= 1
\end{align}
\begin{align}
\Rightarrow \hat I^{(2p)}(\nu) &=\frac {2^{3-\nu}\pi\Gamma(\nu-1)}{(\nu-2)\Gamma(\frac{n-1} 2+p)\Gamma(\frac{n-1} 2-p)} \cdot \frac{\Gamma(\frac{\nu-1} 2-p)}{2^{p}\Gamma(\frac{\nu-1} 2)} \cdot \frac{(2p!)}{2^p p!}\\
 &= \frac{\sqrt{\pi}(2p)!}{2^{2p}p!} \frac {\Gamma((\nu-2)/2)} {\Gamma(\frac{\nu-1}2+p)}
\end{align}

\subsubsection{any collinearity and $-k,-l\in\mathbbm N_0$}
If $-k,-l\in\mathbbm N_0$ $I_{n}^{(k,l)}$ can always be reduced in a straight forward manner to combinations of $\hat I^{(q)}(n)$ and this way one finds\cite[Ch. 5]{Bojak:2000eu}\cite[App. C]{PhysRevD.40.54}:
\begin{align}
I^{(0,0)}_{n} &= \hat I^{(0)}(n-1) \cdot \hat I^{(0)}(n) = \frac{2\pi}{n-3}\\
I^{(0,0)}_{4} &= 2\pi\\
I^{(-1,0)}_{n} &= \hat I^{(0)}(n-1) \cdot (a\hat I^{(0)}(n)+b\hat I^{(1)}(n)) = \frac{2\pi a}{n-3}\\
I^{(-1,0)}_{4} &= 2\pi a \\
I^{(0,-1)}_{n} &= \hat I^{(0)}(n-1) \cdot (A\hat I^{(0)}(n) + B\hat I^{(1)}(n)) + C\hat I^{(1)}(n-1)\hat I^{(0)}(n)\\
 &= \frac{2\pi A}{n-3}\\
I^{(0,-1)}_{4} &=2\pi A\\
I^{(-2,0)}_{n} &= \hat I^{(0)}(n-1) \cdot (a^2\hat I^{(0)}(n)+2ab\hat I^{(1)}(n) + b^2 \hat I^{(2)}(n))\\
 &= 2\pi\left(\frac{a^2(n-1)+b^2}{(n-1)(n-3)}\right)\\
I^{(-2,0)}_{4} &= 2\pi(a^2 + b^2/3) \\
I^{(0,-2)}_{n} &= \hat I^{(0)}(n-1) \cdot (A^2\hat I^{(0)}(n) + B^2\hat I^{(2)}(n)) + C^2\hat I^{(2)}(n-1)\hat I^{(0)}(n+2) \\
 &= 2\pi\left(\frac{A^2(n-1)+B^2+C^2}{(n-1)(n-3)}\right)\\
I^{(0,-2)}_{4} &= 2\pi(A^2+(B^2+C^2)/3) \\
I^{(-1,-1)}_{n} &= \hat I^{(0)}(n-1) \cdot (a A\hat I^{(0)}(n) + b B \hat I^{(2)}(n)) = 2\pi\left(\frac{aA(n-1)+bB}{(n-1)(n-3)}\right)\\
I^{(-1,-1)}_{4} &= 2\pi(aA + bB/3)
\end{align}

\subsubsection{single collinear a}
If $-l\in\mathcal N$ one finds:
\begin{align}
\hat I_{a}^{(k,q)}(\nu) &= \int\limits_0^\pi\!\frac{\sin^{\nu-3}t}{(1-\cos(t))^k}\cos^q(t)\, dt \\
 &= \int\limits_0^\pi\!\frac{\sin^{\nu-3}(t)}{(1-\cos^2(t))^k}\cos^q(t)(1+\cos(t))^k\, dt\\
 &=\int\limits_0^\pi\!\sin^{\nu-3-2k}(t)\cos^q(t)(1+\cos(t))^k\, dt\\
 &= \sum\limits_{l=0}^k\binom{k}{l}\hat I^{(q+l)}(\nu-2k)
\end{align}

this way one finds\cite[Ch. 5]{Bojak:2000eu}\cite[App. C]{PhysRevD.40.54}:
\begin{align}
I^{(1,0)}_{a,n} &= \frac 1 a\hat I^{(0)}(n-1) \cdot \hat I^{(0)}(n-2)\\
 &= \frac {2\pi}{a(n-4)}\\
I^{(1,-1)}_{a,n} &= \frac 1 a\hat I^{(0)}(n-1)\cdot \left(A\hat I^{(0)}(n-2)+B\hat I^{(2)}(n-2)\right)\\
 &= \frac {2\pi}{a}\frac{(A(n-3)+B)}{(n-3)(n-4)} \approx \frac {2\pi}{a}\left(\frac{A+B}\epsilon - 2B + O(\epsilon)\right)\\
I^{(1,-2)}_{a,n} &= \frac 1 a\left(\hat I^{(0)}(n-1)\cdot \left(A^2\hat I^{(0)}(n-2)+(B^2+2AB)\hat I^{(2)}(n-2)\right) + C^2\hat I^{(2)}(n-1)\hat I^{(0)}(n)\right)\\
 &= \frac {2\pi}{a}\left(\frac {A^2}{n-4} + \frac {2AB + B^2}{(n-4)(n-3)} + \frac {C^2}{(n-3)(n-2)}\right)\\
 &\approx \frac {2\pi}{a}\left(\frac{(A+B)^2}{\epsilon}+\frac{C^2}{2}-2AB-B^2+O(\epsilon)\right)
\end{align}
\begin{align}
I^{(2,0)}_{a,n} &= \frac 1 {a^2}\hat I^{(0)}(n-1) \cdot \left(\hat I^{(0)}(n-4) + \hat I^{(2)}(n-4)\right)\\
 &= \frac {2\pi}{a^2(n-6)} \approx -\frac {\pi}{a^2} + O(\epsilon)\\
I^{(2,-1)}_{a,n} &= \frac 1 {a^2}\hat I^{(0)}(n-1) \cdot \left(A\left(\hat I^{(0)}(n-4) + \hat I^{(2)}(n-4)\right) + 2B\hat I^{(2)}(n-4)\right)\\
 &= \frac {2\pi}{a^2}\left(\frac{A}{n-6}+\frac{2B}{(n-6)(n-4)}\right)\approx -\frac{2\pi}{a^2}\left(\frac{B}{\epsilon} + \frac{A+B} 2\right) + O(\epsilon)\\
I^{(2,-2)}_{a,n} &= \frac 1 {a^2}\left(\hat I^{(0)}(n-1)\cdot \left(A^2(\hat I^{(0)}(n-4)+\hat I^{(2)}(n-4))+4AB\hat I^{(2)}(n-4) \right.\right.\nonumber\\
 &\hspace{20pt}\left.\left. + B^2(\hat I^{(2)}(n-4)+\hat I^{(4)}(n-4))\right) + C^2\hat I^{(2)}(n-1)(\hat I^{(0)}(n-2) + \hat I^{(2)}(n-2))\right)\\
 &= \frac {2\pi}{a^2}\left(\frac {A^2}{n-6}+\frac{4AB}{(n-6)(n-4)} + \frac{B^2 n}{(n-6)(n-4)(n-3)} + \frac{C^2}{(n-4)(n-3)} \right) \\
 &\approx \frac {2\pi}{a^2}\left(\frac{-2AB-2B^2+C^2}{\epsilon}+\frac{B^2-A^2}{2}-AB-C^2+O(\epsilon)\right)\\
\end{align}

It is\cite[Ch. 5]{Bojak:2000eu}:
\begin{align}
I_{a,n}^{(1,1)} &= \frac{\pi}{a(A+B)}\left(\frac 2 \epsilon + \ln\left(\frac{(A+B)^2}{A^2-B^2-C^2}\right) \right) + O(\epsilon) \\
I_{a,n}^{(2,1)} &= \frac{\pi}{a^2(A+B)}\left(\frac{B^2+AB+C^2}{(A+B)^2}\left(\frac 2 \epsilon + \ln\left(\frac{(A+B)^2}{A^2-B^2-C^2}\right)\right) \right.\nonumber\\
 &\hspace{60pt}\left. - \frac{2C^2}{(A+B)^2} - 1\right) + O(\epsilon)
\end{align}
From this are the following integrals derived:
\begin{align}
I_{a,n}^{(1,2)} &=-\DeriveP A {I_{a,n}^{(1,1)}} \\
 &= \frac{\pi}{a(A+B)^2}\left(\frac 2 \epsilon + \ln\left(\frac{(A+B)^2}{A^2-B^2-C^2}\right) + \frac{2A(A+B)}{A^2-B^2-C^2} -2 \right) + O(\epsilon) \\
I_{a,n}^{(2,2)} &=-\DeriveP A {I_{a,n}^{(2,1)}} \\
 &= \frac{\pi}{a^2(A+B)^2}\left(\frac{2B^2+2AB+3C^2}{(A+B)^2}\left(\frac 2 \epsilon + \ln\left(\frac{(A+B)^2}{A^2-B^2-C^2}\right)\right)\right.\nonumber\\
 &\hspace{80pt}\left. +\frac{2A^2}{A^2-B^2-C^2} - \frac{8C^2}{(A+B)^2} -3 \right) + O(\epsilon)
\end{align}

\subsubsection{double collinear}
as said in \cite[Ch. 5]{Bojak:2000eu}: if $0\leq -\frac{C}{A},\frac B A \leq 1$ use \cite[eq. A11]{van_neerven_dimensional_1986} with $\cos\kappa = -\frac B A$:
\begin{equation}
I_{aA,n}^{(k,l)} = \frac{2\pi 2^{-(k+l)}}{a^kA^l}\frac{\Gamma(1+\epsilon)}{\Gamma^2(1+\epsilon/2)} B(1+\frac \epsilon 2 - k, 1+ \frac \epsilon 2 -l) \pFq 2 1 \left(k,l;1+\frac \epsilon 2; \frac{A-B}{2A}\right)
\end{equation}

\subsubsection{non collinear}
If $-l\in\mathcal N$ the $\theta_2$ integration can be performed using the integral helper and the problem reduces then to the following integral:
\begin{align}
&\hat I_{0,\cos}^{(k,q,p)}(\epsilon) \nonumber\\
&= \int\limits_0^\pi\!d\theta_1\, \frac{\sin^{1+\epsilon}(\theta_1)\sin^q(\theta_1) \cos^p(\theta_1)}{(a+b\cos(\theta_1))^k}\\
&= \frac 1 {2a^k}\left((1+(-1)^p)B\left(\frac{2+q+\epsilon}{2},\frac{1+p}{2}\right)\pFq 3 2 \left(\frac{1+k}{2},\frac k 2,\frac{1+p}{2};\frac{1}{2},\frac{3+q+p+\epsilon}{2};\frac{b^2}{a^2}\right)\right.\nonumber\\
 &\hspace{20pt}\left. \frac b a k(-1+(-1)^p)B\left(\frac{2+q+\epsilon}{2},\frac{2+p}{2}\right)\pFq 3 2\left(\frac{1+k} 2,\frac{2+k}{2},\frac{2+p}{2};\frac{3}{2},\frac{4+q+p+\epsilon}{2};\frac{b^2}{a^2}\right) \right)
\end{align}
for $k=1$ this simplifies to
\begin{align}
&\hat I_{0,\cos}^{(1,q,p)}(\epsilon) \nonumber\\
&= \int\limits_0^\pi\!d\theta_1\, \frac{\sin^{1+\epsilon}(\theta_1)\sin^q(\theta_1) \cos^p(\theta_1)}{(a+b\cos(\theta_1))}\\
&= \frac 1 {2a}\left((1+(-1)^p)B\left(\frac{2+q+\epsilon}{2},\frac{1+p}{2}\right)\pFq 2 1 \left(1,\frac{1+p}{2};\frac{3+q+p+\epsilon}{2};\frac{b^2}{a^2}\right)\right.\nonumber\\
 &\hspace{20pt}\left. \frac b a (-1+(-1)^p)B\left(\frac{2+q+\epsilon}{2},\frac{2+p}{2}\right)\pFq 2 1\left(1,\frac{2+p}{2};\frac{4+q+p+\epsilon}{2};\frac{b^2}{a^2}\right) \right)
\end{align}
\textit{TODO: structure does NOT match \cite[Ch. 5]{Bojak:2000eu} - neither A,B,C nor $\epsilon$}  \fxerror{fix to Bojak}

For $I_{0,n}^{1,1}$ one finds\cite[Ch. 5]{Bojak:2000eu}:
\begin{align}
I_{0,n}^{1,1} &= \frac{\pi}{\sqrt X}\ln\left(\frac{aA - bB + \sqrt X}{aA - bC - \sqrt X}\right)\\
X &= (aB - bA)^2 - (a^2-b^2)C^2
\end{align}

\subsection{needed set in matrix element}
define a shortcut:
\begin{equation}
\left(\mathcal V(x,y)\right)_{(k,l)} = x^{-2+k} y^{-2+l} \qquad k,l = \{0,1,2,3\}
\end{equation}

It is
\begin{equation}
A_1 = \sum_{k,l=0}^{3} \left(\mathcal C_{A_1}\right)_{(k,l)} {t'}^{-2+k} {u_7}^{-2+l} = \tr(\mathcal C_{A_1} \mathcal V(t',u_7)^t)
\end{equation}
and we will thus need the integrals
\begin{equation}
\left(\mathcal I_{A_1}\right)_{(k,l)} = \int\!d\Omega_n\,\left(\mathcal V(t',u_7)\right)_{(k,l)}
\end{equation}
with
\begin{align}
a(t') = -b(t') &= -2\omega_1\omega_2 &&= -\frac{s_4(s_4-u_1)}{2(s_4+m^2)}\\
A(u_7) &= q^2-2q_0E_1 &&= q^2-\frac{(s_4+2m^2)(s+u_1)}{2(s_4+m^2)}\\
B(u_7) &= -2\omega_2(\abs{\vec p_2}\cos\psi-\omega_1) &&=\frac {s_4}{2}\left(1-\frac{s+u_1}{s_4+m^2}+\frac{s-q^2-t_1}{s_4-u_1}\right)\\
C(u_7) &= -2\omega_2\abs{\vec p_2}\sin\psi
\end{align}
that is $I_{a,n}^{(-1\ldots 2,-1\ldots 2)}$. With this we get
\begin{equation}
\int\!d\Omega_n\,A_1 = \tr(\mathcal C_{A_1} \left(\mathcal I_{A_1}\right)^t)
\end{equation}
%\begin{align}
%\int\!d\Omega_n &= \frac{2\pi}{n-3}\\
%\int\!d\Omega_n\,t' &= \frac{2\pi}{n-3} (-2\omega_1\omega_2) &&= -\frac{\pi}{n-3}\cdot\frac{s_4(s_4-u_1)}{s_4+m^2}\\
%\int\!d\Omega_n\,u_7 &= \frac{2\pi}{n-3}(q^2-2q_0E_1) &&=\frac{\pi}{n-3}\left(2q^2+\frac{(s_4+2m^2)(s+u_1)}{2(s_4+m^2)}\right)\\
%\int\!d\Omega_n\,\frac 1 {t'} &= \frac{2\pi}{n-4} \frac 1 {-2\omega_1\omega_2} &&= -\frac{4\pi}{n-4}\cdot\frac{s_4+m^2}{s_4(s_4-u_1)}\\
%\end{align}

It is
\begin{equation}
A_2 = \sum_{k,l=0}^{3} \left(\mathcal C_{A_2}\right)_{(k,l)} {s_5}^{-2+k} {u'}^{-2+l} = \tr(\mathcal C_{A_2} \mathcal V(s_5,u')^t)
\end{equation}
and we will thus need the integrals
\begin{equation}
\left(\mathcal I_{A_2}\right)_{(k,l)} = \int\!d\Omega_n\,\left(\mathcal V(s_5,u')\right)_{(k,l)}
\end{equation}
but as both $s_5$ and $u'$ are of $[ABC]$ type we have to apply partial fractioning, following the ideas of \cite[Ch. 5]{Bojak:2000eu}. It is 
\begin{equation}
(\ref{eq:MonCon3s5up}): \qquad s_5 = s-q^2+t'+u'
\end{equation}
so end up with a form of $\mathcal V(p+q,q)$ where $p$ is $[ab]$ and $q$ and $p+q$ are $[ABC]$. The aim is then to get to a form with fractions of $\frac p q$ and/or $\frac {p+q} p$ and indeed this can be achieved. Define
\begin{equation}
\mathcal T =\!\left(\!\!
\begin{array}{cccc}
\{-2,1,2,1\} & \{1,\hphantom{-} 0,-1,-1\} & \{0,0,0,1\} & \{0,0,1,-1\}\\
\{-1,1,1,0\} & \{1,-1,\hphantom{-} 0,\hphantom{-} 0\}  & \{0,0,1,0\} & \{0,0,1,-1\}\\
\{\hphantom{-} 0,1,0,0\}  & \{1,\hphantom{-} 0,\hphantom{-} 0,\hphantom{-} 0\}   & \{1,0,0,0\} & \{0,0,1,-1\}\\
\{\hphantom{-} 1,1,0,0\}  & \{1,\hphantom{-} 1,\hphantom{-} 0,\hphantom{-} 0\}   & \{1,1,0,0\} & \{0,0,1,-1\}
\end{array}\!\!
\right)
\end{equation}
\begin{equation}
\left(\mathcal W(x,y)\right)_{(k,l)} = x^{-2+p_x(k+l)} y^{-2+p_y(k+l)}
\end{equation}
\begin{equation}
p_x(s) = \left\{\begin{array}{ll}k+l&\text{if }k+l\leq 3\\ 3 &\text{else}\end{array}\right.
\qquad
p_y(s) = \left\{\begin{array}{ll}0&\text{if }k+l\leq 3\\ k+l-3 &\text{else}\end{array}\right.
\end{equation}
\begin{equation}
\Rightarrow \mathcal W(x,y) = \!\left(\!\!
\begin{array}{cccc}
x^{-2}y^{-2} & x^{-1}y^{-2} & y^{-2} & xy^{-2}\\
x^{-1}y^{-2} & y^{-2} & xy^{-2} & xy^{-1} \\
y^{-2} & xy^{-2} & xy^{-1} & x\\
xy^{-2} & xy^{-1} & x & xy
\end{array}\!\!
\right)
\end{equation}
\begin{equation}
\left(\mathcal{W}^*(p,q)\right)_{(k,l)} = \left\{\frac q p\mathcal W(p,q),\mathcal W(p,q),\frac {p+q} p\mathcal W(p,p+q),\mathcal{W}(p,p+q)\right\}_{(k,l)}
\end{equation}
we then find:
\begin{equation}
\left(\mathcal V(p+q,q)\right)_{(k,l)} = \mathcal T_{(k,l)}\cdot \mathcal W^*(p,q)_{(k,l)}
\end{equation}
where the equation has to be read separate for each $(k,l)$, i.e. ``$\cdot$`` applies to the scalar $4x4$-product of the $\{\}$s. As $\mathcal W^t = \mathcal W$, $\mathcal W$ has 10 unique entries and thus for $\mathcal W^*$ are 40 unique integrals needed: $I_0^{(-1\ldots 3,-2\ldots 2)}$.

