align $k_1$ to z-axis:
\begin{align}
k_1 &= (\omega_1,0,0,\omega_1, \hat 0)\\
q &= (q_0,0,\abs{\vec p_2}\sin\psi,\abs{\vec p_2}\cos\psi-\omega_1, \hat 0)\\
p_2 &= (E_2,0,\abs{\vec p_2}\sin\psi,\abs{\vec p_2}\cos\psi, \hat 0)
\end{align}

light quark masses are already fixed: $k_1^2 = 0 = k_2^2$

constraints:
\begin{align}
q_0+\omega_1 & &&=E_1+E_2+\omega_2 \label{eq:PSConIMomCon}\\
m^2 &= p_1^2 &&= E_1^2 - \omega_2^2 \label{eq:PSConIp1}\\
m^2 &= p_2^2 &&= E_2^2 - \abs{\vec p_2}^2 \label{eq:PSConIp2} \\
q^2 & &&= q_0^2 - \abs{\vec p_2}^2 + 2\abs{\vec p_2}\omega_1\cos\psi-\omega_1^2 \label{eq:PSConIq}\\
s &= (q+k_1)^2 &&= (q_0+\omega_1)^2 - \abs{\vec p_2}^2 \label{eq:PSConIs}\\
t &= (k_1-p_2)^2 &&= (\omega_1-E_2)^2-\abs{\vec p_2}^2+2\abs{\vec p_2}\omega_1\cos\psi-\omega_1^2 \label{eq:PSConIt}\\
u &= (q-p_2)^2 &&= (q_0-E_2)^2 - \omega_1^2 \label{eq:PSConIu}
\end{align}

solve:
\begin{align}
(\ref{eq:PSConIs}) - (\ref{eq:PSConIq}) + (\ref{eq:PSConIt}) - (\ref{eq:PSConIp2}) + (\ref{eq:PSConIu}) &= s-q^2+t-m^2+u\\
 &= s_4+m^2 = (E_1+\omega_2)^2 \label{eq:PSConIs4}\\
(\ref{eq:PSConIt}) + (\ref{eq:PSConIu}) - (\ref{eq:PSConIq}) &= t+u-q^2 = -2(E_1+\omega_2)E_2\\
\Rightarrow E_2 &= -\frac{t+u-q^2}{2\sqrt{s_4+m^2}} =\frac{s-s_4-2m^2}{2\sqrt{s_4+m^2}} \label{eq:PSConIE2}\\
(\ref{eq:PSConIs4})\land (\ref{eq:PSConIp1}) \Rightarrow \omega_2 &= \frac{s_4}{2\sqrt{s_4+m^2}} \label{eq:PSConIom2} \\
(\ref{eq:PSConIs4})\Rightarrow E_1 &= \frac{s_4+2m^2}{2\sqrt{s_4+m^2}} \label{eq:PSConIE1} \\
(\ref{eq:PSConIs})+(\ref{eq:PSConIu})-(\ref{eq:PSConIp2}) &= s+u-m^2 =2q_0(E_1+\omega_2)\\
\Rightarrow q_0 &= \frac{s+u_1}{2\sqrt{s_4+m^2}} \label{eq:PSConIq0}\\
(\ref{eq:PSConIt}) - (\ref{eq:PSConIq}) &= t-q^2 = (\omega_1-E_2)^2 - q_0^2\\
\Rightarrow \omega_1 &= \frac{s'+t_1}{2\sqrt{s_4+m^2}} = \frac{s_4-u_1}{2\sqrt{s_4+m^2}}\label{eq:PSConIom1}\\
(\ref{eq:PSConIp2}) \Rightarrow \abs{\vec p_2} &= \sqrt{E_2^2 - m^2} = \frac {\sqrt{(s-s_4)^2-4sm^2}} {2\sqrt{s_4+m^2}}\label{eq:PSConIabsp2}\\
(\ref{eq:PSConIq}) \Rightarrow \cos\psi &= \frac{q^2-q_0^2+\abs{\vec p_2}^2+\omega_1^2}{2\abs{\vec p_2}\omega_1}\\
 &= \frac {(u_1+m^2)(t_1-s')-(m^2-q^2-t_1)(s'+t_1)} {(s'+t_1)\sqrt{(s-s_4)^2-4sm^2}}\label{eq:PSConIabcos}\\
\Rightarrow \sin\psi &= 2\frac{\sqrt{s_4+m^2}\sqrt{m^2s'^2+q^2t_1(s'+t_1)-s't_1u_1}}{(s'+t_1)\sqrt{(s-s_4)^2-4sm}}
\end{align}

\begin{align}
&&t' &= -2k_1k_2 = -2\omega_1\omega_2(1-\cos\theta_1)\\
&&u_6 &= - 2k_1p_1 = -2\omega_1(E_1 + \omega_2\cos\theta_1)\\
(\ref{eq:MomCon3wk1}): &&0 &= s+t_1+t'+u_6-q^2\quad\checkmark
\end{align}

$t'$ is the only variable that can get collinear (for $-q^2 > 0$).

\begin{align}
&&s_3 &= 2k_2p_2 = 2\omega_2(E_2-\abs{\vec p_2}(\cos\psi\cos\theta_1+\sin\psi\sin\theta_1\cos\theta_2))\\
&&s_5 &= (p_1+p_2)^2 = 2m^2+2p_1p_2\\
&& &= 2(m^2+E_1E_2+\omega_2\abs{\vec p_2}(\cos\psi\cos\theta_1+\sin\psi\sin\theta_1\cos\theta_2))\\
(\ref{eq:MomCon3wp2}): &&0 &= s_3+s_5+t_1+u_1-q^2\quad\checkmark
\end{align}

\begin{align}
&&u' &=(q-k_2)^2 = q^2-2qk_2\\
&& &= q^2-2(q_0\omega_2 -\omega_2(\abs{\vec p_2}\cos\psi-\omega_1)\cos\theta_1-\omega_2\abs{\vec p_2}\sin\psi\sin\theta_1\cos\theta_2)\\
&&u_7 &= q^2-2qp_1\\
&& &=q^2 - 2(q_0E_1 +\omega_2(\abs{\vec p_2}\cos\psi-\omega_1)\cos\theta_1 + \omega_2\abs{\vec p_2}\sin\psi\sin\theta_1\cos\theta_2)\\
(\ref{eq:MomCon3wq}): &&0 &=s+u_1+u_7+u'-2q^2\quad\checkmark
\end{align}
